\chapter{Theory for LASSO in high dimensions}
Part of this chapter follows \textit{Statistics for High-Dimensional Data} by Peter BÃ¼hlmann and Sara van de Geer.

\section{Assuming the truth is linear}
In this section, we assume that there exists some ``true value" that would make the parameter \(\bta\) fit the observations to the predictions perfectly. We call this ideal parameter vector \(\bta^0\). However, we work with an underdetermined system: there are more variables than equations, or in our context, there are more parameters than observations \((\ie p>n)\).

We define $\btahat$ as follows
\begin{equation}
    \label{eqn: beta hat (LASSO)}
    \btahat:=\arg \min _{\bta}\left\{ \frac{\|\Y-\X \bta\|_{2}^{2}}{n}+\lambda\|\bta\|_{1} \right\}
\end{equation}

\begin{lemma}[Basic Inequality]
    \label{lemma: basic inequality}
    \[
        \frac{\| \X (\btahat-\bta^{0})\|_{2}^{2}}{n} + \lambda\|\btahat\|_{1} \leq 2 \frac{\varepsilon^{T} \X (\btahat-\bta^{0})}{n}+\lambda \| \bta^{0} \|_{1}
    \]
\end{lemma}
\begin{proof}
    By definition of $\btahat$, we have that
    \[
        \forall \bta \quad \frac{\| \Y-\X \btahat \|_{2}^{2}}{n} + \lambda \| \btahat \|_{1} \leq \frac{\|\Y-\X \bta \|_{2}^{2}}{n}+\lambda \| \bta \|_{1}
    \]
    In particular for $\bta = \bta^0$ we have
    \[
        \frac{\| \Y-\X \btahat \|_{2}^{2}}{n}+\lambda\| \btahat \|_{1} \leq \frac{ \| \Y-\X \bta^0\|_{2}^{2}}{n}+\lambda \| \bta^0\|_{1}
    \]
    We now replace $\Y$ using equation \eqref{eqn: linear model (matrix)}:
    \begin{align*}
                 & \frac{\|\Y  - \X \btahat \|_{2}^{2}}{n} + \lambda \| \btahat\|_{1} \leq \frac{\| \Y  - \X \bta^0 \|_2^2}{n}+\lambda\|\bta^{0}\|_{1}                                                     \\
        \implies &
        \frac{\| (\X \bta^0 + \eps) - \X \btahat \|_{2}^{2}}{n}+\lambda\| \btahat \|_{1} \leq \frac{ \| (\X \bta^0 + \eps)-\X \bta^0\|_{2}^{2}}{n}+\lambda \| \bta^0\|_{1}                                 \\
        \implies &
        \frac{\langle \X ( \bta^0 - \btahat) + \eps, \X ( \bta^0 - \btahat) + \eps \rangle}{n}+\lambda \| \btahat \|_{1} \leq \frac{ \| \eps \|_{2}^{2}}{n}+\lambda \| \bta^0\|_{1}                        \\
        \implies &
        \frac{\| \X (\bta^0 - \btahat) \| _2^2 + \| \eps \|_2^2 + 2 \langle \X ( \bta^0 - \btahat),  \eps \rangle}{n}+\lambda \| \btahat \|_{1} \leq \frac{ \| \eps \|_{2}^{2}}{n}+\lambda \| \bta^0\|_{1} \\
        \implies &
        \frac{\| \X (\btahat - \bta^0) \| _2^2}{n} + \lambda \| \btahat \|_{1} \leq \frac{2 \langle \X ( \btahat - \bta^0),  \eps \rangle}{n} + \lambda \| \bta^0\|_{1}                                    \\
        \implies &
        \frac{\| \X (\btahat - \bta^0) \| _2^2}{n} + \lambda \| \btahat \|_{1} \leq \frac{2 \eps^T \X ( \btahat - \bta^0)}{n} + \lambda \| \bta^0\|_{1}                                                    \\
    \end{align*}
    This completes the proof.
\end{proof}
We define \(\mathscr{T}\) as follows
\[
    \mathscr{T} := \left\{ \max _{1 \leq j \leq p} 2 \frac{\left| \varepsilon^{T} \mathbf{X}^{(j)}\right|}{n} \leq \lambda_{0}\right\}
\]
\(\mathscr{T}\) gives us a useful upper bound if we can find a value of \(\lambda_0\) such that \(\mathscr{T}\) has probability close to 1. Lemma \ref{lemma: value for lambda_0} will give us such an upper bound.

\begin{lemma}
    \label{lemma: value for lambda_0}
    Assume \(\forall \; j = 1, \ldots, p, \; \sgmhat_j^2 = 1 \) and for all $t > 0$ and let
    \[
        \lambda_{0}:=2 \sgm \sqrt{\frac{t^{2}+2 \log p}{n}}
    \]
    we have
    \[
        \mathbb{P}(\mathscr{T}) \geq 1-2 \exp \left[ \frac{-t^{2}}{2} \right]
    \]
\end{lemma}
\begin{proof}
    We define
    \[
        V_{j} := \frac{\varepsilon^{T} \mathbf{X}^{(j)}}{\sqrt{n \sgm^{2}}}
    \]
    Then we have
    \begin{align}
        \nonumber
        \mathbb{P}(\mathscr{T})
         & = \P \left( \max _{1 \leq j \leq p} 2 \frac{\left| \varepsilon^{T} \mathbf{X}^{(j)}\right|}{n} \leq 2 \sgm \sqrt{\frac{t^{2}+2 \log p}{n}}  \right) \\
        \nonumber
         & =
        \P \left( \max _{1 \leq j \leq p} \left| \frac{\varepsilon^{T} \mathbf{X}^{(j)}}{\sqrt{n \sgm^{2}}} \right| \leq \sqrt{t^{2}+2 \log p}  \right)        \\
        \nonumber
         & =
        \P \left( \max _{1 \leq j \leq p} | V_{j} | \leq \sqrt{t^{2}+2 \log p}  \right)                                                                        \\
        \nonumber
         & = 1 - \P \left( \max _{1 \leq j \leq p} | V_{j} | > \sqrt{t^{2}+2 \log p}  \right)                                                                  \\
        \nonumber
         & = 1 - \P \left( \bigcup_{j = 1}^{p} \left\{ | V_{j} | > \sqrt{t^{2}+2 \log p}  \right\} \right)                                                     \\
        \nonumber
         & \geq 1 - \sum_{j = 1}^{p} \P \left( | V_{j} | > \sqrt{t^{2}+2 \log p}  \right)                                                                      \\
        \label{eqn: proof lemma 6.2.}
         & \geq 1 - p \; \P \left( | V_{j} | > \sqrt{t^{2}+2 \log p}  \right)
    \end{align}
    Now, let us define $\zeta := \sqrt{t^{2}+2 \log p}$. Since $V_j$ is $\mathscr{N} (0,1)$-distributed and $\zeta > 0$, it follows that

    \begin{align*}
        \mathbb{P}(V_j > \zeta) & = \frac{1}{\sqrt{2\pi}} \int_\zeta^{\infty} e^{-y^2/2} dy                   \\
                                & < \frac{1}{\sqrt{2\pi}} \int_\zeta^{\infty} \frac{y}{\zeta} e^{-y^2 / 2} dy \\
                                & = \frac{1}{\zeta \sqrt{2\pi}} \int_\zeta^{\infty} y e^{-y^2 / 2} dy         \\
                                & = \frac{1}{\zeta\sqrt{2\pi}} e^{-\zeta^2/2}                                 \\
    \end{align*}
    We note that $p \geq 2 \implies \zeta \sqrt{2 \pi} \geq 1$ therefore
    \[
        \mathbb{P}(V_j > \zeta) <  e^{-\zeta^2/2}
    \]
    Moreover by symmetry of the $\mathscr{N} (0,1)$ distribution,

    \begin{align*}
        \mathbb{P} (|V_j| > \zeta) & = 2 \mathbb{P} (V_j > \zeta) \\
                                   & < 2 e^{-\zeta^2/2}           \\
    \end{align*}
    Inserting this result into \eqref{eqn: proof lemma 6.2.} we obtain

    \begin{align*}
        \mathbb{P}(\mathscr{T}) & \geq 1 - p \; \P \left( | V_{j} | > \sqrt{t^{2}+2 \log p}  \right) \\
                                & \geq 1 - p \; \frac{2}{p} \exp \left[ \frac{- t^{2}}{2} \right]    \\
                                & = 1 - 2 \exp \left[ \frac{- t^{2}}{2} \right]                      \\
    \end{align*}
\end{proof}

\begin{corollary}[Consistency of the LASSO] % Corollary 6.1
    Assume $\sgmhat^2_j = 1$ for all \(j = 1, \ldots, p\). For some \(t > 0\), we define the regularization parameter as
    \[
        \lambda := 4 \sgmhat \sqrt{\frac{t^2 + 2 \log p}{n}}
    \]
    where $\sgmhat$ is an estimator of $\sgm$. \\
    Then with probability at least $1 - \alpha$, where
    \[
        \alpha := 2 \exp \left[ \frac{- t^{2}}{2} \right] + \P (\{\sgmhat \leq \sgm\})
    \]
    we have
    \[
        2 \frac{\| \X (\btahat - \bta^0)\|_2^2}{n} \leq 3 \lambda \| \bta^0 \|_1
    \]
\end{corollary}
\begin{proof}
    Recall that we defined
    \[
        \mathscr{T} := \left\{ \max _{1 \leq j \leq p} 2 \frac{\left| \varepsilon^{T} \mathbf{X}^{(j)}\right|}{n} \leq \lambda_{0}\right\}
    \]
    and lemma \ref{lemma: value for lambda_0}, we know that
    \[
        \lambda_{0} = 2 \sgm \sqrt{\frac{t^{2}+2 \log p}{n}} \implies \mathbb{P}(\mathscr{T}) \geq 1-2 \exp \left[ \frac{-t^{2}}{2} \right]
    \]
    So if \(\sgmhat > \sgm\), replacing the latter by the former will result in a weaker statement, which therefore still holds, \ie
    \[
        \lambda_{0} = 2 \sgmhat \sqrt{\frac{t^{2}+2 \log p}{n}} \implies \mathbb{P}(\mathscr{T}) \geq 1-2 \exp \left[ \frac{-t^{2}}{2} \right]
    \]
    Now if we are on \(\T\), starting with the basic inequality \ref{lemma: basic inequality}:
    \begin{align*}
                 & \frac{\| \X (\btahat-\bta^{0})\|_{2}^{2}}{n} + 2\lambda_0 \|\btahat\|_{1} \leq 2 \frac{\eps^{T} \X (\btahat-\bta^{0})}{n} + 2\lambda_0 \| \bta^{0} \|_{1}                                             \\
        \implies & \frac{\| \X (\btahat-\bta^{0})\|_{2}^{2}}{n} \leq \underbrace{2 \frac{\eps^{T} \X (\btahat - \bta^{0})}{n}}_{\text{bounded on } \T} + 2 \lambda_0 \left( \| \bta^{0} \|_{1} - \|\btahat\|_{1} \right) \\
        \implies & \frac{\| \X (\btahat-\bta^{0})\|_{2}^{2}}{n} \leq \lambda_0 ( \underbrace{\|\btahat - \bta^{0} \|_1 - \|\btahat\|_{1}}_{\leq \| \bta^{0} \|_{1}} + 2 \| \bta^{0} \|_{1} )                             \\
        \implies & \frac{\| \X (\btahat-\bta^{0})\|_{2}^{2}}{n} \leq 3 \lambda_0 \| \bta^{0} \|_{1}
    \end{align*}
    Therefore with \(\lambda = 2 \lambda_0 = 4 \sgmhat \sqrt{\frac{t^2 + 2 \log p}{n}}\), we obtain the desired result. This occurs if we are on \( \T \) and \(\sgmhat > \sgm\), which means that it doesn't occur with probability
    \begin{align*}
         & \P(\neg \T \cup \{ \sgmhat \leq \sgm \})                                                          \\
         & = \P(\neg \T) + \P(\{ \sgmhat \leq \sgm \}) - \P(\neg \T \cap \{ \sgmhat \leq \sgm \})            \\
         & \leq \P(\neg \T) + \P(\{ \sgmhat \leq \sgm \})                                                    \\
         & = 1 - \P(\T) + \P(\{ \sgmhat \leq \sgm \})                                                        \\
         & \leq 1 - \left( 1 - 2 \exp \left[ \frac{- t^{2}}{2} \right] \right) + \P(\{ \sgmhat \leq \sgm \}) \\
         & = 2 \exp \left[ \frac{- t^{2}}{2} \right] + \P(\{ \sgmhat \leq \sgm \})
    \end{align*}
    which concludes the proof.
\end{proof}

\begin{lemma} % Lemma 6.3.
    \label{eqn: lemma 6.3.}
    We have on $\mathscr{T}$, with $\lambda \geq 2 \lambda_{0}$,
    \begin{equation*}
        2\frac{ \|\mathbf{X} (\btahat-\bta^{0} ) \|_{2}^{2}}{n} + \lambda \|\btahat_{S_{0}^{c}} \|_{1} \leq 3 \lambda \|\btahat_{S_{0}}-\bta_{S_{0}}^{0} \|_{1}
    \end{equation*}
\end{lemma}
\begin{proof}
    We start with the Basic Inequality
    \[
        \frac{\| \X (\btahat-\bta^{0})\|_{2}^{2}}{n} + \lambda\|\btahat\|_{1} \leq 2 \frac{\varepsilon^{T} \X (\btahat-\bta^{0})}{n}+\lambda\|\bta^{0}\|_{1}
    \]
    Now since we are on $\mathscr{T}$ and since $2 \lambda_0 \leq \lambda$
    \[
        \frac{\| \X (\btahat-\bta^{0})\|_{2}^{2}}{n} + \lambda\|\btahat\|_{1} \leq \lambda_0 \|\btahat-\bta^{0}\|_1 + \lambda\|\bta^{0}\|_{1}
    \]
    \[
        2 \frac{\| \X (\btahat-\bta^{0})\|_{2}^{2}}{n}+2 \lambda\|\btahat\|_{1} \leq \lambda \|\btahat-\bta^{0} \|_{1}+2 \lambda \|\bta^{0} \|_{1}
    \]
    Let $\bta_{j, S}:=\bta_{j} 1\{j \in S\}$. We use the triangle inequality on the left hand side
    \begin{align*}
        \|\btahat\|_{1}
         & = \|\btahat_{S_{0}} \|_{1} + \|\btahat_{S_{0}^{c}} \|_{1}                                                \\
         & = \|\bta_{S_{0}}^{0} - \bta_{S_{0}}^{0} + \btahat_{S_{0}} \|_{1} + \|\btahat_{S_{0}^{c}} \|_{1}          \\
         & \geq \|\bta_{S_{0}}^{0} \|_{1} - \|\btahat_{S_{0}}-\bta_{S_{0}}^{0} \|_{1}+ \|\btahat_{S_{0}^{c}} \|_{1}
    \end{align*}
    whereas on the right hand side
    \begin{align*}
        \|\btahat-\bta^{0} \|_{1}
         & =  \| (\btahat_{S_{0}} + \btahat_{S_{0}^{c}}) - (\bta_{S_{0}}^{0} + \underbrace{\bta_{S_{0}^{c}}^0)}_{=0} \|_{1} \\
         & =  \| \btahat_{S_{0}}-\bta_{S_{0}}^{0} \|_{1} + \|\btahat_{S_{0}^{c}} \|_{1}
    \end{align*}
    Injecting these two results, we get that
    \begin{align*}
                 & 2 \frac{\| \X (\btahat-\bta^{0})\|_{2}^{2}}{n} + 2 \lambda\|\btahat\|_{1} \leq \lambda \|\btahat-\bta^{0} \|_{1}+2 \lambda \|\bta^{0} \|_{1}                                                                                                \\
        \implies & 2 \frac{\| \X (\btahat-\bta^{0})\|_{2}^{2}}{n} + 2 \lambda \left( \|\bta_{S_{0}}^{0} \|_{1} - \|\btahat_{S_{0}}-\bta_{S_{0}}^{0} \|_{1}+ \|\btahat_{S_{0}^{c}} \|_{1} \right)                                                               \\
                 & \leq \lambda \left( \| \btahat_{S_{0}}-\bta_{S_{0}}^{0} \|_{1} + \|\btahat_{S_{0}^{c}} \|_{1} \right) + 2 \lambda \|\bta^{0} \|_{1}                                                                                                         \\
        \implies & 2 \frac{\| \X (\btahat-\bta^{0})\|_{2}^{2}}{n} + 2 \lambda \|\underbrace{\bta_{S_{0}}^{0}}_{= \bta^0} \|_{1} + \lambda \|\btahat_{S_{0}^{c}} \|_{1} \leq 3 \lambda \| \btahat_{S_{0}}-\bta_{S_{0}}^{0} \|_{1} + 2 \lambda \|\bta^{0} \|_{1} \\
        \implies & 2\frac{ \|\mathbf{X} (\btahat-\bta^{0} ) \|_{2}^{2}}{n} + \lambda \|\btahat_{S_{0}^{c}} \|_{1} \leq 3 \lambda \|\btahat_{S_{0}}-\bta_{S_{0}}^{0} \|_{1}
    \end{align*}
\end{proof}

\begin{definition}[Compatibility condition]
    We say that the compatibility condition is met for the set $S_{0}$, if for some $\phi_{0}>0$, and for all $\bta$ satisfying $ \|\bta_{S_{0}^{c}} \|_{1} \leq 3 \|\bta_{S_{0}} \|_{1}$, it holds that
    \begin{equation}
        \left\| \bta_{S_{0}} \right\|_{1}^{2} \leq \left(\bta^{T} \Sgmhat \bta\right) \frac{s_{0}}{\phi_{0}^{2}}
    \end{equation}
\end{definition}

\begin{theorem}[Theorem 6.1.]
    Suppose the compatibility condition holds for $S_{0}$. Then on $\mathscr{T}$, we have for $\lambda \geq 2 \lambda_{0}$,
    $$
        \frac{\|\mathbf{X}(\btahat-\bta^{0})\|_{2}^{2}}{n}+\lambda\|\btahat-\bta^{0}\|_{1} \leq 4 \lambda^{2} \frac{s_{0}}{\phi_{0}^{2}}
    $$
\end{theorem}
\begin{proof}
    Using Lemma \ref{eqn: lemma 6.3.} we have that
    \begin{align*}
         & \quad 2 \frac{\|\mathbf{X}(\btahat-\bta^{0})\|_{2}^{2}}{n} + \lambda\|\btahat-\bta^{0}\|_{1}                                                                                                    \\
         & = 2 \frac{\|\mathbf{X}(\btahat-\bta^{0})\|_{2}^{2}}{n} + \lambda \| \btahat_{S_0} + \btahat_{S_{0}^{c}} - \bta^{0}_{S_0} - \underbrace{\bta^{0}_{S_0^c}}_{=0} \|_{1}                            \\
         & = 2 \frac{\|\mathbf{X}(\btahat-\bta^{0})\|_{2}^{2}}{n} + \lambda \| \btahat_{S_0} - \bta^{0}_{S_0} \|_{1} + \lambda \| \btahat_{S_{0}^{c}} \|_1 \quad \textit{(by lemma \ref{eqn: lemma 6.3.})} \\
         & \leq 4 \lambda \|\btahat_{S_{0}} - \bta_{S_{0}}^{0} \|_{1}                                                                                                                                      \\
         & = 4 \lambda \sqrt{\left( \btahat_{S_{0}} - \bta_{S_{0}}^{0} \right)^{T} \Sgmhat \left( \btahat_{S_{0}} - \bta_{S_{0}}^{0}  \right) s_{0} / \phi_{0}^{2}}                                        \\
         & \leq \sqrt{\left( \btahat_{S_{0}} - \bta_{S_{0}}^{0} \right)^{T} \X^T \X \left( \btahat_{S_{0}} - \bta_{S_{0}}^{0}  \right)} \frac{4 \lambda \sqrt{s_{0}}}{\phi_{0} \sqrt{n}}                   \\
         & \leq \| \X ( \btahat_{S_{0}} - \bta_{S_{0}}^{0} ) \|_2 \frac{4 \lambda \sqrt{s_{0}}}{\phi_{0} \sqrt{n}}                                                                                         \\
         & \leq \| \X ( \btahat_{S_{0}} - \bta_{S_{0}}^{0} ) \|^2_2 + \frac{4 \lambda^2 s_{0}}{\phi^2_{0} n}                                                                                               \\
    \end{align*}
    Where the last inequality follows from $4uv \leq u^2 + 4v^2$.
\end{proof}


\section{Linear approximation of the truth}

Now $\mathbf{Y} :=\mathbf{f}^{0} + \eps$, therefore $\mathbb{E} [\mathbf{Y}] :=\mathbf{f}^{0}$.


\begin{lemma}[New version of the Basic Inequality]
    $\forall \bta^* \in \R^p$ we have
    \begin{equation}
        \frac{\|\X \btahat - \mathbf{f}^0 \|_{2}^{2}}{n} + \lambda\| \btahat \|_{1} \leq \frac{2 \eps^T \X (\btahat - \bta^*)}{n} + \lambda \| \bta^*\|_{1} + \frac{\|\X \bta^* - \mathbf{f}^0\|_{2}^{2}}{n}
    \end{equation}
\end{lemma}
\begin{proof}
    By definition of $\btahat$, we have that
    $$
        \forall \bta \quad \frac{\| \Y -\X \btahat \|_{2}^{2}}{n} + \lambda \| \btahat \|_{1} \leq \frac{\|\Y-\X \bta \|_{2}^{2}}{n}+\lambda \| \bta \|_{1}
    $$
    In particular for $\bta = \bta^*$ we have
    $$
        \forall \bta^* \quad \frac{\| \Y -\X \btahat \|_{2}^{2}}{n} + \lambda \| \btahat \|_{1} \leq \frac{\|\Y-\X \bta^* \|_{2}^{2}}{n}+\lambda \| \bta^* \|_{1}
    $$
    Since $\Y = \mathbf{f}^0 + \eps$:
    \begin{align*}
                 & \frac{\|\Y  - \X \btahat \|_{2}^{2}}{n} + \lambda \| \btahat\|_{1} \leq \frac{\| \Y  - \X \bta^* \|_2^2}{n}+\lambda\|\bta^{*}\|_{1}                                                       \\
        \implies &
        \frac{\| (\mathbf{f}^0 - \X \btahat ) + \eps \|_{2}^{2}}{n} + \lambda\| \btahat \|_{1} \leq \frac{ \| (\mathbf{f}^0 - \X \bta^*) + \eps \|_{2}^{2}}{n}+\lambda \| \bta^*\|_{1}                       \\
        \implies &
        \frac{\langle (\mathbf{f}^0 - \X \btahat ) + \eps, (\mathbf{f}^0 - \X \btahat ) + \eps \rangle}{n} + \lambda\| \btahat \|_{1}                                                                        \\
                 & \leq \frac{ \langle (\mathbf{f}^0 - \X \bta^*) + \eps, (\mathbf{f}^0 - \X \bta^*) + \eps \rangle}{n}+\lambda \| \bta^*\|_{1}                                                              \\
        \implies &
        \frac{\|\mathbf{f}^0 - \X \btahat \|_{2}^{2} + \| \eps \|_{2}^{2} + 2\langle \mathbf{f}^0 - \X \btahat, \eps \rangle}{n} + \lambda\| \btahat \|_{1}                                                  \\
                 & \leq \frac{\|\mathbf{f}^0 - \X \bta^* \|_{2}^{2} + \| \eps \|_{2}^{2} + 2\langle \mathbf{f}^0 - \X \bta^*, \eps \rangle}{n}+\lambda \| \bta^*\|_{1}                                       \\
        \implies &
        \frac{\|\X \btahat - \mathbf{f}^0 \|_{2}^{2}}{n} + \lambda\| \btahat \|_{1} \leq \frac{2 \eps^T \X (\btahat - \bta^*)}{n} + \lambda \| \bta^*\|_{1} + \frac{\|\X \bta^* - \mathbf{f}^0\|_{2}^{2}}{n} \\
    \end{align*}
\end{proof}

\begin{lemma}[New version of Lemma 6.3.]
    We have on $\mathscr{T}$, with $\lambda \geq 4 \lambda_{0}$,
    \begin{equation}
        \label{eqn: new version of lemma 6.3.}
        \frac{4 \|\mathbf{X} \btahat-\mathbf{f}^0\|_{2}^{2}}{n} + 3 \lambda \| \btahat_{S^{c}_{*}} \|_{1} \leq 5 \lambda \| \btahat_{S_{*}} - \bta_{S_{*}}^{*} \|_{1} + \frac{4 \|\mathbf{X} \bta^{*} - \mathbf{f}^{0} \|_{2}^{2}}{n}
    \end{equation}
    where $S_* := \{ j: \bta_j^* \neq 0 \}$.
\end{lemma}
\begin{proof}
    We start with the Basic Inequality
    $$
        \frac{\|\X \btahat - \mathbf{f}^0 \|_{2}^{2}}{n} + \lambda\| \btahat \|_{1} \leq  \frac{2 \eps^T \X (\btahat - \bta^*)}{n} + \lambda \| \bta^*\|_{1} + \frac{\|\X \bta^* - \mathbf{f}^0\|_{2}^{2}}{n}
    $$
    Now since we are on $\mathscr{T}$ and since $4 \lambda_0 \leq \lambda$
    \begin{align*}
                 & \frac{\|\X \btahat - \mathbf{f}^0 \|_{2}^{2}}{n} + \lambda\| \btahat \|_{1} \leq  \frac{2 \eps^T \X (\btahat - \bta^*)}{n} + \lambda \| \bta^*\|_{1} + \frac{\|\X \bta^* - \mathbf{f}^0\|_{2}^{2}}{n} \\
        \implies &
        4 \frac{\| \X \btahat - \mathbf{f}^0 \|_{2}^{2}}{n} + 4 \lambda\| \btahat \|_{1} \leq \lambda \| \btahat - \bta^* \|_{1} + 4 \lambda \| \bta^*\|_{1} + 4\frac{\|\X \bta^* - \mathbf{f}^0\|_{2}^{2}}{n}           \\
    \end{align*}
    We use the triangle inequality on the left hand side
    \begin{align*}
        \|\btahat\|_{1}
         & = \|\btahat_{S_{*}} \|_{1} + \|\btahat_{S_{*}^{c}} \|_{1}                                                \\
         & = \|\bta_{S_{*}}^{*} - \bta_{S_{*}}^{*} + \btahat_{S_{*}} \|_{1} + \|\btahat_{S_{*}^{c}} \|_{1}          \\
         & \geq \|\bta_{S_{*}}^{*} \|_{1} - \|\btahat_{S_{*}}-\bta_{S_{*}}^{*} \|_{1}+ \|\btahat_{S_{*}^{c}} \|_{1}
    \end{align*}
    whereas on the right hand side
    \begin{align*}
        \|\btahat-\bta^{*} \|_{1}
         & =  \| (\btahat_{S_{*}} + \btahat_{S_{*}^{c}}) - (\bta_{S_{*}}^{*} + \underbrace{\bta_{S_{*}^{c}}^*}_{=0}) \|_{1} \\
         & =  \| \btahat_{S_{*}}-\bta_{S_{*}}^{*} \|_{1} + \|\btahat_{S_{*}^{c}} \|_{1}
    \end{align*}
    Injecting these two results, we get that
    \begin{align*}
                 & 4 \frac{\| \X \btahat - \mathbf{f}^0 \|_{2}^{2}}{n} + 4 \lambda\| \btahat \|_{1} \leq \lambda \| \btahat - \bta^* \|_{1} + 4 \lambda \| \bta^*\|_{1} + 4\frac{\|\X \bta^* - \mathbf{f}^0\|_{2}^{2}}{n} \\
        \implies &
        4 \frac{\| \X \btahat - \mathbf{f}^0 \|_{2}^{2}}{n} + 4 \lambda \left( \|\bta_{S_{*}}^{*} \|_{1} - \|\btahat_{S_{*}}-\bta_{S_{*}}^{*} \|_{1}+ \|\btahat_{S_{*}^{c}} \|_{1} \right)                                \\
                 & \leq \lambda \left( \| \btahat_{S_{*}}-\bta_{S_{*}}^{*} \|_{1} + \|\btahat_{S_{*}^{c}} \|_{1} \right) + 4 \lambda \| \bta^*\|_{1} + 4\frac{\|\X \bta^* - \mathbf{f}^0\|_{2}^{2}}{n}                    \\
        \implies &
        4 \frac{\| \X \btahat - \mathbf{f}^0 \|_{2}^{2}}{n} + 4 \lambda \| \underbrace{\bta_{S_{*}}^{*}}_{= \bta^{*}} \|_{1} + 3 \lambda\|\btahat_{S_{*}^{c}} \|_{1}                                                      \\
                 & \leq 5 \lambda \| \btahat_{S_{*}}-\bta_{S_{*}}^{*} \|_{1} + 4 \lambda \| \bta^*\|_{1} + 4\frac{\|\X \bta^* - \mathbf{f}^0\|_{2}^{2}}{n}                                                                \\
        \implies &
        4 \frac{\| \X \btahat - \mathbf{f}^0 \|_{2}^{2}}{n} + 3 \lambda\|\btahat_{S_{*}^{c}} \|_{1} \leq 5 \lambda \| \btahat_{S_{*}}-\bta_{S_{*}}^{*} \|_{1} + 4\frac{\|\X \bta^* - \mathbf{f}^0\|_{2}^{2}}{n}           \\
    \end{align*}
\end{proof}

% Compare  equation \eqref{eqn: lemma 6.3.} and equation \eqref{eqn: new version of lemma 6.3.}. We have that 

\begin{definition}[Compatibility condition for general sets]
    We say that the compatibility condition holds for the set $S$, if for some constant $\phi(S)>0,$ and for all $\bta,$ with $\left\|\bta_{S^{c}}\right\|_{1} \leq$ $3\left\|\bta_{S}\right\|_{1},$ one has
    $$
        \left\|\bta_{S}\right\|_{1}^{2} \leq\left(\bta^{T} \sgmhat \bta\right)\frac{|S|}{\phi^{2}(S)}
    $$
\end{definition}

We define $\mathscr{S}$ as the collection of sets $S$ for which the compatibility condition holds.

\begin{definition}[The oracle]
    We define the oracle $\bta^{*}$ as
    $$
        \bta^{*} = \arg \min_{\bta: S_{\bta} \in \mathscr{S}} \left\{ \frac{ \left\| \X \bta - \f^{0} \right\|_{2}^{2}}{n} + \frac{4 \lambda^{2} s_{\bta}}{\phi^{2}\left(S_{\bta}\right)}\right\}
    $$
    where $S_{\bta}:=\left\{j: \bta_{j} \neq 0\right\}$, $s_{\bta}:=\left|S_{\bta}\right|$ denotes the cardinality of $S_{\bta}$ and the factor 4 in the right hand side comes from choosing $\lambda \geq \lambda_0$.
\end{definition}




