\chapter{Introduction}
\section{The first section}
\subsection{The first subsection}

\begin{equation}
    \label{def: linear model (matrix)}
    \Y = \X \beta + \eps
\end{equation}

We define $\hat \beta$ as follows
\begin{equation}
    \label{not: beta hat}
    \hat{\beta}:=\arg \min _{\beta}\left\{\frac{\|\Y-\X \beta\|_{2}^{2}}{n}+\lambda\|\beta\|_{1}\right\}
\end{equation}

\begin{lemma}[Basic Inequality]
    $$\frac{\| \X (\hat{\beta}-\beta^{0})\|_{2}^{2}}{n} + \lambda\|\hat{\beta}\|_{1} \leq 2 \frac{\varepsilon^{T} \X (\hat{\beta}-\beta^{0})}{n}+\lambda\|\beta^{0}\|_{1}$$
\end{lemma}
\begin{proof}
    By definition of $\hat \beta$, we have that
    $$
        \forall \beta \quad \frac{\| \Y-\X \hat \beta \|_{2}^{2}}{n} + \lambda \| \hat \beta \|_{1} \leq \frac{\|\Y-\X \beta \|_{2}^{2}}{n}+\lambda \| \beta \|_{1}
    $$
    In particular for $\beta = \beta^0$ we have
    $$
        \frac{\| \Y-\X \hat \beta \|_{2}^{2}}{n}+\lambda\| \hat \beta \|_{1} \leq \frac{ \| \Y-\X \beta^0\|_{2}^{2}}{n}+\lambda \| \beta^0\|_{1}
    $$
    We now replace $\Y$ using equation \eqref{def: linear model (matrix)}.
    \begin{align*}
                 & \frac{\|\Y  - \X \hat{\beta} \|_{2}^{2}}{n} + \lambda \| \hat{\beta}\|_{1} \leq \frac{\| \Y  - \X \beta^0 \|_2^2}{n}+\lambda\|\beta^{0}\|_{1}                                                       \\
        \implies &
        \frac{\| (\X \beta^0 + \eps) - \X \hat \beta \|_{2}^{2}}{n}+\lambda\| \hat \beta \|_{1} \leq \frac{ \| (\X \beta^0 + \eps)-\X \beta^0\|_{2}^{2}}{n}+\lambda \| \beta^0\|_{1}                                   \\
        \implies &
        \frac{\| \X ( \beta^0 - \hat \beta) + \eps \|_{2}^{2}}{n} + \lambda\| \hat \beta \|_{1} \leq \frac{ \| \X ( \beta^0 - \beta^0) + \eps \|_{2}^{2}}{n}+\lambda \| \beta^0\|_{1}                                  \\
        \implies &
        \frac{\langle \X ( \beta^0 - \hat \beta) + \eps, \X ( \beta^0 - \hat \beta) + \eps \rangle}{n}+\lambda \| \hat \beta \|_{1} \leq \frac{ \| \eps \|_{2}^{2}}{n}+\lambda \| \beta^0\|_{1}                        \\
        \implies &
        \frac{\| \X (\beta^0 - \hat \beta) \| _2^2 + \| \eps \|_2^2 + 2 \langle \X ( \beta^0 - \hat \beta),  \eps \rangle}{n}+\lambda \| \hat \beta \|_{1} \leq \frac{ \| \eps \|_{2}^{2}}{n}+\lambda \| \beta^0\|_{1} \\
        \implies &
        \frac{\| \X (\hat \beta - \beta^0) \| _2^2}{n} + \lambda \| \hat \beta \|_{1} \leq \frac{2 \langle \X ( \hat \beta - \beta^0),  \eps \rangle}{n} + \lambda \| \beta^0\|_{1} \\
        \implies &
        \frac{\| \X (\hat \beta - \beta^0) \| _2^2}{n} + \lambda \| \hat \beta \|_{1} \leq \frac{2 \eps^T \X ( \hat \beta - \beta^0)}{n} + \lambda \| \beta^0\|_{1} \\
    \end{align*}
\end{proof}